Examples.v
@@ -74,4 +74,171 @@ Proof with ellipsis.
         destruct (X =? X) eqn:E...
         eapply ieq_iff_neq...
 Qed.
+
+(* 
+  Proposition 8.1 of Brookes - laws of parallel programming
+*)
+Theorem law_of_parallel_programming_1: 
+  forall c, 
+    [|c|] ~ [|c ; skip|].
+Proof with ellipsis.
+  split; repeat intro.
+   - apply SmSeq.
+    destruct a.
+    { apply nil_not_in_CSemantics in H... }
+    assert (
+      exists a' p', p :: a = a' ++ [p']
+    ).
+    { 
+      clear H c.
+      remember (p :: a) as l.
+      generalize dependent a.
+      generalize dependent p.
+      clean_induction l...
+      invert Heql.
+      destruct a0.
+      - exists [], p...
+      - assert (p0 :: a0 = p0 :: a0)...
+        clean_apply_in IHl H.
+        destruct H as [a' [p']].
+        exists (p :: a'), p'...
+      Unshelve.
+      auto. auto.
+    }
+    destruct H0 as [a' [[s s']]]. rewrite H0 in *. 
+    clear H0 a p.
+    replace (a' ++ [(s, s')])
+      with (a' ++ [(s, s')] ++ [])...
+    apply sm_mumbly with s'. simpl.
+    replace (a' ++ [(s, s'); (s', s')])
+      with ((a' ++ [(s, s')]) ++ [(s', s')]) 
+      by (rewrite <- app_assoc; eauto).
+    apply sm_self. 
+    exists (a' ++ [(s, s')]), [(s', s')].
+    repeat split...
+    eapply SmSkip. apply sm_self...
+  - invert H.
+    apply CSemantics_stuttery_mumbly.
+    eapply sm_closure_implication'...
+    clear H3 a. intros ts [ts1 [ts2 [H []]]].
+    subst.
+    invert H0. induction H1.
+    + invert H0.
+      replace (ts1 ++ [(s, s)])
+        with (ts1 ++ [(s, s)] ++ [])...
+      apply sm_stuttery.
+      rewrite <- app_nil_end...
+    + rewrite app_assoc in *.
+      apply sm_stuttery...
+    + rewrite app_assoc in *.
+      eapply sm_mumbly...
+Qed.
+
+Theorem law_of_parallel_programming_2: 
+  forall c1 c2 c3, 
+    [|(c1; c2); c3|] ~ [|c1; (c2; c3)|].
+Proof with ellipsis.
+  intros. split; repeat intro.
+  - apply CSemantics_equiv'.
+    apply CSemantics_equiv' in H.
+    apply sm_closure_implication
+      with [|(c1; c2); c3|]'...
+    clear H a. intros ts H.
+    invert H. destruct H3 as [ts1 [ts2 [H []]]].
+    invert H. destruct H5 as [ts1' [ts1'' [H []]]].
+    subst.
+    rewrite <- app_assoc.
+    apply SmSeq'.
+    exists ts1', (ts1'' ++ ts2). repeat split...
+    apply SmSeq'...
+  - apply CSemantics_equiv'.
+    apply CSemantics_equiv' in H.
+    apply sm_closure_implication
+      with [|c1; (c2; c3)|]'...
+    clear H a. intros ts H.
+    invert H. destruct H3 as [ts1 [ts2 [H []]]].
+    invert H0. destruct H5 as [ts2' [ts2'' [H0 []]]].
+    subst.
+    rewrite app_assoc.
+    apply SmSeq'.
+    exists (ts1 ++ ts2'), ts2''. repeat split...
+    apply SmSeq'...
+Qed.
+
+Lemma semantics_implication_via':
+  forall c1 c2,
+    [|c1|]' |= [|c2|]'
+      ->
+    [|c1|] |= [|c2|].
+Proof with ellipsis.
+  intros. intros ts H0.
+  apply sm_closure_implication in H.
+  apply CSemantics_equiv' in H0.
+  apply H in H0.
+  apply CSemantics_equiv'...
+Qed.
     
+(* 
+  Brookes only states the first direction,
+    as he is referring to rough-grain semantics,
+    in which the second program allows
+    context switches between the evaluation of
+    b1 and b2, but the first program doesn't.
+  However, in fine-grained semantics this
+    distinction is lost, and we have full
+    equivalence.
+*)
+Theorem law_of_parallel_programming_3: 
+  forall b1 b2 c1 c2,
+    [|if b1 && b2 then c1 else c2 end|]
+      ~
+    [|if b1 then if b2 then c1 else c2 end else c2 end|].
+Proof with ellipsis.
+  intros. split; intros.
+  - eapply semantics_implication_via'; 
+      [ |eassumption].
+    clear H a. intros ts H.
+    invert H; 
+      destruct H4 as [ts1 [ts2 [? []]]]; subst;
+      invert H.
+    + destruct H5 as [ts1' [ts1'' [? []]]]. subst.
+      rewrite <- app_assoc.
+      apply SmIfTrue'.
+      exists ts1', (ts1'' ++ ts2). repeat split...
+      apply SmIfTrue'...
+    + apply SmIfFalse'...
+    + destruct H5 as [ts1' [ts1'' [? []]]]. subst.
+      rewrite <- app_assoc.
+      apply SmIfTrue'.
+      exists ts1', (ts1'' ++ ts2). repeat split...
+      apply SmIfFalse'...
+  - eapply semantics_implication_via'; 
+      [ |eassumption].
+    clear H a. intros ts H.
+    invert H; 
+      destruct H4 as [ts1 [ts2 [? []]]]; subst.
+    + invert H0;
+        destruct H5 as [ts1' [ts1'' [? []]]]; subst;
+        rewrite app_assoc.
+      * apply SmIfTrue'.
+        repeat eexists...
+        apply SmAndTrue'...
+      * apply SmIfFalse'.
+        repeat eexists...
+        apply SmAndTrue'...
+    + apply SmIfFalse'. 
+      repeat eexists...
+      apply SmAndFalse'...
+Qed.
+
+Theorem law_of_parallel_programming_4: 
+  forall b c,
+    [|while b do c end|]
+      ~
+    [|if b then c; while b do c end else skip end|].
+Proof with ellipsis.
+  intros; split; intros;
+    apply TT_equiv_Semantics;
+    apply while_equiv_if_while;
+    apply TT_equiv_Semantics...
+Qed.
